high2/Zeta.High.Blum.fsti
@@ -1,0 +1,79 @@
+module Zeta.High.Blum
+
+open Zeta.SeqAux
+open Zeta.Interleave
+open Zeta.MultiSet
+open Zeta.MultiSetHashDomain
+open Zeta.Time
+open Zeta.GenKey
+open Zeta.EAC
+open Zeta.GenericVerifier
+open Zeta.Generic.Interleave
+open Zeta.Generic.Blum
+open Zeta.High.Interleave
+open Zeta.High.TSLog
+
+(* for an eac ts log, if the eac state of a key k is instore, the count of blum evicts
+ * is the same of blum adds for that key for any epoch *)
+val lemma_evict_add_count_same
+  (#app #n:_)
+  (ep: epoch)
+  (il: eac_log app n)
+  (gk:key app):
+  Lemma (requires (let bk = to_base_key gk in
+                   let es = eac_state_of_key bk il in
+                   EACInStore? es))
+        (ensures (size (k_add_set ep gk il) = size (k_evict_set ep gk il)))
+
+val eac_instore_addb_diff_elem
+  (#app #n:_)
+  (itsl: its_log app n)
+  (i: seq_index itsl{let itsli = prefix itsl i in
+                     is_blum_add itsl i /\
+                     is_eac itsli /\
+                     (let e = index itsl i in
+                      let k = add_slot e in
+                      let es = eac_state_of_key k itsli in
+                      EACInStore? es)})
+  : (be':ms_hashfn_dom app{let ep = be'.t.e in
+                           let as = add_set ep itsl in
+                           let es = evict_set ep itsl in
+                           let be = blum_add_elem itsl i in
+                           mem be' as > mem be' es /\
+                           be.t.e = ep})
+
+val eac_evictedm_addb_diff_elem
+  (#app #n:_)
+  (itsl: its_log app n)
+  (i:seq_index itsl{let itsli = prefix itsl i in
+                    is_blum_add itsl i /\
+                    is_eac itsli /\
+                    (let e = index itsl i in
+                     let k = add_slot e in
+                     let es = eac_state_of_key k itsli in
+                     EACEvictedMerkle? es)})
+  : (be':ms_hashfn_dom app{let ep = be'.t.e in
+                           let as = add_set ep itsl in
+                           let es = evict_set ep itsl in
+                           let be = blum_add_elem itsl i in
+                           mem be' as > mem be' es /\
+                           be.t.e = ep})
+
+val eac_evictedb_addb_diff_elem
+  (#app #n:_)
+  (itsl: its_log app n)
+  (i: seq_index itsl{let itsli = prefix itsl i in
+                     let itsli' = prefix itsl (i + 1) in
+                     is_blum_add itsl i /\
+                     is_eac itsli /\
+                     not (is_eac itsli') /\
+                     (let e = index itsl i in
+                      let k = add_slot e in
+                      let es = eac_state_of_key k itsli in
+                      EACEvictedBlum? es)})
+  : (be':ms_hashfn_dom app{let ep = be'.t.e in
+                           let as = add_set ep itsl in
+                           let es = evict_set ep itsl in
+                           let be = blum_add_elem itsl i in
+                           mem be' as > mem be' es /\
+                           be.t.e = ep})
